theories/normalization.v
@@ -1,0 +1,174 @@
+Set Warnings "-notation-overridden,-parsing,-deprecated-hint-without-locality".
+From Coq Require Import Strings.String.
+From stdpp Require Import gmap list.
+From logical_relation Require Import relation syntax_stlc opsem_stlc.
+
+Implicit Types Γ : context.
+Implicit Types τ : ty.
+
+Definition substitution := list (string*val).
+Implicit Types γ : substitution.
+Fixpoint domain γ :=
+  match γ with
+    | nil => []
+    | (x,v)::γ' => x::(domain γ')
+  end.
+
+Fixpoint substitute γ e :=
+  match γ with
+  | nil => e
+  | (x,v)::γ' => substitute γ' (subst_term x (of_val v) e)
+  end.
+
+Definition normalize_to_v e v :=
+  is_val v -> e ~>* v.
+
+Definition normalize e :=
+  exists v, normalize_to_v e v.
+Notation "⇓ e" := (normalize e) (at level 99).
+
+Fixpoint sn (τ : ty) (e : expr) :=
+ match τ with
+ | Ty_Bool => (∅ ⊢ e ∈ Bool) /\ ⇓ e
+ | Ty_Arrow t1 t2 =>
+    (∅ ⊢ e ∈ (t1 -> t2))
+    /\ (⇓ e)
+    /\ (forall e', sn t1 e' -> sn t2 <{ e e' }> )
+ end.
+
+Definition sem_subst γ Γ :=
+  Forall (fun x => sn (match (Γ !! x) with
+                      | None => Ty_Bool
+                      | Some t => t
+                    end)
+                  (substitute γ (expr_var x)))
+    (domain γ).
+  (* dom Γ = domain γ. *)
+Notation " γ ⊨ Γ" := (sem_subst γ Γ) (at level 99).
+Lemma sn_safe : forall τ e, sn τ e -> ⇓ e.
+Proof.
+  intros.
+  destruct τ; simpl in H ; firstorder.
+Qed.
+
+Lemma substitution_lemma Γ γ τ e :
+  Γ ⊢ e ∈ τ ->
+  γ ⊨ Γ ->
+  (typing_judgment ∅ (substitute γ e) τ).
+Admitted.
+
+Lemma sn_backward τ e e':
+ (∅ ⊢ e ∈ τ) ->
+ e ~> e' ->
+ (sn τ e' -> sn τ e).
+Admitted.
+
+Lemma sn_backward_star τ e e':
+ (∅ ⊢ e ∈ τ) ->
+ e ~>* e' ->
+ (sn τ e' -> sn τ e).
+Admitted.
+
+Lemma sn_forward τ e e':
+ (∅ ⊢ e ∈ τ) ->
+ e ~> e' ->
+ (sn τ e -> sn τ e').
+Admitted.
+
+Lemma sn_forward_star τ e e':
+ (∅ ⊢ e ∈ τ) ->
+ e ~>* e' ->
+ (sn τ e -> sn τ e').
+Admitted.
+
+Lemma sn_well_typed τ e: sn τ e -> (∅ ⊢ e ∈ τ).
+Proof.
+  intros. destruct τ; simpl in *;firstorder.
+Qed.
+
+Lemma substitute_true γ :
+(substitute γ <{ true }> ) = <{true}>.
+Admitted.
+Lemma substitute_false γ :
+(substitute γ <{ false }> ) = <{false}>.
+Admitted.
+
+Lemma substitute_app γ e e' :
+(substitute γ <{ e e' }>) =
+  expr_app (substitute γ <{ e }>) (substitute γ <{ e' }>).
+Admitted.
+
+Lemma substitute_if γ e e1 e2 :
+(substitute γ <{ if e then e1 else e2 }>) =
+  expr_if (substitute γ <{ e }>) (substitute γ <{ e1 }>) (substitute γ <{ e2 }>).
+Admitted.
+
+Lemma fundamental : forall Γ γ τ e,
+  (Γ ⊢ e ∈ τ) ->
+  γ ⊨ Γ ->
+  sn τ (substitute γ e).
+Proof.
+  induction 1 ; simpl in *; intros.
+  - (* true *)
+    split; rewrite substitute_true; auto.
+    eexists; intro; eapply star_refl.
+  - (* false *)
+    split; rewrite substitute_false; auto.
+    eexists; intro; eapply star_refl.
+  - (* var *) admit.
+  - (* lam *)
+    split.
+    apply substitution_lemma with (Γ := Γ);auto.
+    split. admit.
+    intros.
+    admit.
+  - (* app *)
+    pose proof H1 as H2.
+    apply IHtyping_judgment1 in H1
+    ; clear IHtyping_judgment1
+    ; destruct H1 as (IH1_type & IH1_norm & IH1_sn).
+    apply IHtyping_judgment2 in H2; clear IHtyping_judgment2.
+    rewrite substitute_app.
+    by apply IH1_sn.
+  - (* if *)
+    pose proof H2 as H3;
+    pose proof H2 as H4.
+    apply IHtyping_judgment1 in H2
+    ; clear IHtyping_judgment1
+    ; destruct H2 as [H_bool H_norm].
+    apply IHtyping_judgment2 in H3
+    ; clear IHtyping_judgment2.
+    apply IHtyping_judgment3 in H4
+    ; clear IHtyping_judgment3.
+
+    destruct H_norm as [v H_norm].
+    assert (Hv : (substitute γ e) ~>* <{ true }>
+                 \/ (substitute γ e) ~>* <{ false }> ).
+    { admit. }
+    destruct Hv.
+    + (* true *)
+      apply sn_backward_star
+        with (e' := expr_if expr_true (substitute γ e1) (substitute γ e2)).
+      rewrite substitute_if.
+      apply T_If; auto;
+      apply sn_well_typed;auto.
+      rewrite substitute_if.
+      admit.
+      apply sn_backward_star with (e' := (substitute γ e1));auto.
+      admit.
+      apply star_one; auto.
+    + (* false *)
+      apply sn_backward_star
+        with (e' := expr_if expr_false (substitute γ e1) (substitute γ e2)).
+      rewrite substitute_if.
+      apply T_If; auto;
+      apply sn_well_typed;auto.
+      rewrite substitute_if.
+      admit.
+      apply sn_backward_star with (e' := (substitute γ e2));auto.
+      admit.
+      apply star_one; auto.
+Admitted.
+
+
+Lemma well_typed_sn: forall τ e, (∅ ⊢ e ∈ τ) -> sn τ e.
